updated the SpecM.v file with a new interface for SpecM

theories/Ref/SpecM.v
@@ -14,13 +14,272 @@ From EnTree Require Import
      Ref.MRecSpec
 .
 
+From Coq Require Import Lists.List.
+
 From Paco Require Import paco.
+
+From Equations Require Import Equations Signature.
 
 Local Open Scope entree_scope.
 Local Open Scope list_scope.
+
+
+(*
+  should we enfore that A has type universe < entree_u? 
+  can that encode that we want?
+  perhaps no, because the existing code has everything at sort 0, where
+  we will want sort 1,
+
+  types of form forall a b c..., SpecM ... (R a b c ...)
+*)
+Inductive LetRecType : Type@{entree_u + 1} :=
+  | LRT_Ret (R : Type@{entree_u}) : LetRecType
+  | LRT_Fun (A : Type@{entree_u}) (rest : A -> LetRecType) : LetRecType.
+
+(*
+Inductive LetRecTypeArg : LetRecType -> Type :=
+  | LRT_RetArg R : unit -> LetRecTypeArg (LRT_Ret R)
+  | LRT_FunArg A rest (a : A) (b : LetRecTypeArg (rest a) ) : LetRecTypeArg (LRT_Fun A rest).
+*)
+(* defines input type for a lrt event *)
+Fixpoint LRTInput (lrt : LetRecType) : Type@{entree_u} :=
+  match lrt with
+  | LRT_Ret R => unit
+  | LRT_Fun A rest => forall a : A, LRTInput (rest a) 
+  end.
+
+
+Fixpoint LRTOutput lrt : EncodedType (LRTInput lrt) :=
+  match lrt with
+  | LRT_Ret R => fun _ : unit => R
+  | LRT_Fun A rest => fun args =>
+                       forall a : A, LRTOutput (rest a) (args a) end.
+
+#[global] Instance LRTOutputEncoded lrt : EncodedType (LRTInput lrt) := LRTOutput lrt.
+
+Notation function_sigs := (list LetRecType).
+Notation function_stack := (list function_sigs).
+(*
+Inductive call_var : mutual_sigs -> LetRecType -> Type :=
+| VarZ : forall (Γ : mutual_sigs) (lrt : LetRecType), call_var (lrt :: Γ) lrt
+| VarS : forall (Γ : mutual_sigs) (lrt1 lrt2 : LetRecType),
+    call_var Γ lrt1 -> call_var (lrt2 :: Γ) lrt1.
+*)
+(*
+Fixpoint call_var_arg Γ lrt (v : call_var Γ lrt) : Type@{entree_u} :=
+  match v with
+  | VarZ Γ' lrt' => LetRecTypeE lrt'
+  | VarS Γ' lrt1 lrt2 c => call_var_arg _ _ c end.
+*)
+Fixpoint function_sig_index (lrts : function_sigs) (n : nat) : LetRecType :=
+  match lrts with
+  | nil => LRT_Ret void
+  | lrt :: lrts' => 
+      match n with
+      | 0 => lrt
+      | S m => function_sig_index lrts' m end 
+  end.
+(*
+Fixpoint LRTSBodies (lrts : function_sigs) (body_type : LetRecType -> Type) :=
+  match lrts 
+*)
+
+Fixpoint typed_list (l : list Type) : Type :=
+  match l with
+  | nil => unit
+  | h :: t => h * (typed_list t) end.
+
+(* a sort of typed debruijn variable borrowed from one of Steve's developments*)
+Inductive function_var : LetRecType -> function_sigs -> Type :=
+  | VarZ lrt lrts : function_var lrt (lrt :: lrts)
+  | VarS lrt lrt' lrts : function_var lrt lrts -> function_var lrt (lrt' :: lrts).
+
+Fixpoint function_var_index (n : nat) (lrts : function_sigs) : option LetRecType :=
+  match lrts with
+  | nil => None
+  | lrt :: lrts' =>
+      match n with
+      | 0 => Some lrt
+      | S m => function_var_index m lrts' end
+      end.
+
+(*need to figure *)
+
+Inductive SpecM (E : Type) `{EncodedType E} : function_stack -> Type@{entree_u} -> Type := 
+  | RetS Γ A (a : A) : SpecM E Γ A
+  | BindS Γ A B : SpecM E Γ A -> (A -> SpecM E Γ B) -> SpecM E Γ B
+  | IterS Γ A B : (A -> SpecM E Γ (A + B)) -> A -> SpecM E Γ B
+  | TriggerS Γ (e : E) : SpecM E Γ (encodes e)
+  | AssumeS Γ (P : Prop) : SpecM E Γ unit
+  | AssertS Γ (P : Prop) : SpecM E Γ unit
+  | ForallS Γ (A : Set) : SpecM E Γ A
+  | ExistsS Γ (A : Set) : SpecM E Γ A 
+  | CallS Γ lrts lrt (x : function_var lrt lrts) (args : LRTInput lrt) : 
+    SpecM E (lrts :: Γ) (LRTOutput lrt args)
+  | (* I am concerned this is a bit more expressive than necessary,
+                 this bodies function can dispatch on the info of which index it is,
+                 actual CFG's in the language won't do that,
+                 although I suppose extra expressiveness is not necessarily a problem
+                 as long as it does not make the new type too complicated
+               *)
+    MultiFixS Γ lrts 
+              (bodies : forall lrt, function_var lrt lrts -> forall (args : LRTInput lrt),
+                  SpecM E (lrts :: Γ) (LRTOutput lrt args))
+    lrt (x : function_var lrt lrts) : 
+    forall args : LRTInput lrt, SpecM E Γ (LRTOutput lrt args).
+
+Fixpoint LRTsInput (lrts : function_sigs) : Type@{entree_u} :=
+  match lrts with
+  | nil => void
+  | lrt :: lrts' =>
+      LRTInput lrt + (LRTsInput lrts')
+  end.
+
+(* this was a key missing piece I should have seen earlier *)
+Equations LRTinjection (lrt : LetRecType) (lrts : function_sigs) (x : function_var lrt lrts) (args : LRTInput lrt) : LRTsInput lrts  :=
+  LRTinjection lrt (lrt :: lrts) (VarZ lrt lrts) args := inl args;
+  LRTinjection lrt (lrt' :: lrts) (VarS lrt lrt' lrts y) args := inr (LRTinjection lrt lrts y args).
+
+
+Equations LRTsOutput (lrts : function_sigs) (args : LRTsInput lrts) : Type@{entree_u} :=
+  LRTsOutput nil args := match args : void with end;
+  LRTsOutput (lrt :: lrts') (inl args') := LRTOutput lrt args';
+  LRTsOutput (lrt :: lrts') (inr args') := LRTsOutput lrts' args'.
+
+
+Fixpoint function_stackE (E : Type) (Γ : function_stack) : Type@{entree_u} :=
+  match Γ with
+  | nil => E
+  | lrts :: Γ' => LRTsInput lrts + function_stackE E Γ' 
+  end.
+
+Equations function_stackE_encodes (E : Type) `{EncodedType E} (Γ : function_stack) (args : function_stackE E Γ) : Type@{entree_u}:=
+  function_stackE_encodes E nil e := encodes e;
+  function_stackE_encodes E (lrts :: Γ') (inl args') => LRTsOutput lrts args';
+  function_stackE_encodes E (lrts :: Γ') (inr args') => function_stackE_encodes E Γ' args'.
+
+#[global] Instance function_stackE_encodes' (E : Type) `{EncodedType E} (Γ : function_stack) : EncodedType (function_stackE E Γ) :=
+  function_stackE_encodes E Γ.
+
+Equations function_stackE_resum (E : Type) (Γ : function_stack) (e : E) : function_stackE E Γ :=
+  function_stackE_resum E nil e := e;
+  function_stackE_resum E (_ :: Γ') e := inr (function_stackE_resum E Γ' e).
+
+#[global] Instance function_stackE_resum' (E : Type) (Γ : function_stack) : ReSum E (function_stackE E Γ) :=
+  function_stackE_resum E Γ.
+(* TODO: write this with equations *)
+Definition function_stackE_resum_ret (E : Type) `{EncodedType E} (Γ : function_stack) : ReSumRet E (function_stackE E Γ).
+red.  intros e x. induction Γ.
+- cbv in x. exact x.
+- exact (IHΓ x).
+Defined.
+
+#[global] Instance function_stackE_resum_ret' E `{EncodedType E} Γ : ReSumRet E (function_stackE E Γ) :=
+  function_stackE_resum_ret E Γ.
+
+Arguments RetS {_ _ _ _} _.
+Arguments BindS {_ _ _ _ _} _ _.
+Arguments IterS {_ _ _ _ _} _ _.
+Arguments AssumeS {_ _ _}.
+Arguments AssertS {_ _ _}.
+Arguments ExistsS {_ _ _}.
+Arguments ForallS {_ _ _}.
+Arguments TriggerS {_ _ _} _.
+Arguments CallS {_ _ _} _ _ _.
+Arguments MultiFixS {_ _ _ _}.
+
+(* write up the MultiFixS stuff, finish this translation this morning, look more at the haskell in afternoon*)
+
+Definition calls_test (E : Type@{entree_u}) `{EncodedType E} (lrts : function_sigs) Γ (lrt : LetRecType) 
+           (args : LRTInput lrt) (x : function_var lrt lrts) : entree_spec (function_stackE E (lrts :: Γ)) (LRTOutput lrt args).
+simpl. constructor. eapply VisF. Unshelve.
+(*so the problem is injection an LRTInput into an LRTsInput, should rely on function_var *)
+2 : apply (Spec_vis (inl args)).
+eapply (EnTree.trigger (Spec_vis (inl args))) .
+
+Equations denote_SpecM (E : Type@{entree_u}) `{EncodedType E} (Γ : function_stack) (A : Type) (spec : SpecM E Γ A) :
+  entree_spec (function_stackE E Γ) A :=
+  denote_SpecM E Γ A (RetS a) := Ret a;
+  denote_SpecM E Γ A (BindS m k) := EnTree.bind (denote_SpecM E _ _ m) (fun x => denote_SpecM E _ _ (k x));
+  denote_SpecM E Γ A (AssumeS P) := assume_spec P;
+  denote_SpecM E Γ A (AssertS P) := assert_spec P;
+  denote_SpecM E Γ A (ForallS A) := forall_spec A;
+  denote_SpecM E Γ A (ExistsS A) := exists_spec A;
+  denote_SpecM E Γ A (TriggerS e) := trigger e;
+  denote_SpecM E Γ A (CallS lrts lrt x args) := EnTree.trigger (Spec_vis (inl args) );
+  denote_SpecM E Γ A _ := EnTree.spin.
+
+
+Fixpoint denote_SpecM (E : Type@{entree_u}) `{EncodedType E} Γ A (spec : SpecM E Γ A) : 
+  entree_spec (function_stackE E Γ) A :=
+  match spec with
+  | RetS a => Ret a
+  | BindS m k => EnTree.bind (denote_SpecM E _ _ m) (fun x => denote_SpecM E _ _ (k x))
+  | IterS body a => EnTree.iter (fun x => denote_SpecM E _ _ (body x)) a
+  | AssumeS P => assume_spec P
+  | AssertS P => assert_spec P
+  | ForallS A => forall_spec A
+  | ExistsS A => exists_spec A
+  | TriggerS e => trigger e
+  (* I think there is an issue with + vs LRTOutput *)
+  | CallS lrts lrt x args => EnTree.trigger (Spec_vis (inl args) )
+  | _ => EnTree.spin end.
+(*
+
+  | CallS a => (EnTree.trigger (Spec_vis (inl (CallDep _ _ a))))
+  | MrecS A B bodies a => mrec_spec (fun c : call_depE _ _  => 
+                         match c with CallDep _ _ a => denote_SpecM E _ _ (bodies a) end) 
+                               (CallDep _ _ a)
+  end.
+*)
+(* 
+Equations function_stackE_resum_ret (E : Type) `{EncodedType E} (Γ : function_stack) (e : E) (x : encodes (resum e)) :
+  function_stackE_encodes E Γ :=
+  function_stackE_resum_ret E nil e x := x;
+  function_stackE_resum_ret E (_ :: Γ') e x := function_stackE_resum_ret E Γ' e x. *)
+(*write up the translation today *)
+
+(*could be worth proving an isomorphism between function_var lrt lrts and 
+  bound indices
+ *)
+(*
+  | CallS Γ A B (a : A) : SpecM E (ct_intro A B :: Γ) (B a)
+  | MrecS Γ A B (bodies : forall a, SpecM E (ct_intro A B :: Γ) (B a) ) (a : A):
+    SpecM E Γ (B a) *)
+.
+
+(* not sure this is needed
+Fixpoint nat_to_call_var Γ n : option call_var :=
+  match Γ with
+  | nil => None
+  | lrt :: Γ' =>
+      match n with
+      | 0 => Some (VarZ Γ' lrt
+*)
+(* call stack should become a list list lrt 
+   maybe a sort of typed list where each signature has an index
+*)
+
+Instance LetRecTypeEEncodes lrt : EncodedType (LetRecTypeE lrt) := LRTEncodes lrt.
+
+
+Variant callE (lrt : LetRecType) : Type@{entree_u} := Call (a : encodes lrt).
+(* check with eddy to make sure this is right, does this do mutual right? *)
+#[global] Instance callE_encdoes lrt : EncodedType (callE lrt) :=
+  fun _ => encodes lrt.
+
 Variant call_depE (A : Type) (B : A -> Type) : Type@{entree_u} := CallDep (a : A).
 #[global] Instance call_depE_encodes A B : EncodedType (call_depE A B) :=
   fun c => match c with CallDep _ _ a => B a end.
+
+(* should be different for my uses *)
+Fixpoint denote_LetRecType (M : Type -> Type) (lrt : LetRecType) : Type@{entree_u} :=
+  match lrt with
+  | LRT_Ret R => M R (**)
+  | LRT_Fun A rest => forall (a : A), denote_LetRecType M (rest a) end.
+
+#[global] Instance LetRecTypeEncodes : EncodedType LetRecType :=
+  denote_LetRecType.
 
 Variant call_dep_type := 
   ct_intro (A : Type) (B : A -> Type).
@@ -29,9 +288,6 @@ Inductive call_var : call_stack -> call_dep_type -> Type :=
 | VarZ  : forall (G:call_stack) t, call_var (t::G) t
 | VarS  : forall (G:call_stack) u t,
     call_var G t -> call_var (u::G) t.
-
-
-(* call_var is a function into Type entree_u +1*)
 
 Definition call_dep_type_trans (c : call_dep_type) : Type@{entree_u} :=
   match c with ct_intro A B => call_depE A B end.
@@ -45,19 +301,13 @@ Definition call_dep_type_trans (c : call_dep_type) : Type@{entree_u} :=
 Definition uncall {A B} (c : call_depE A B) : A :=
   match c with CallDep _ _ a => a end.
 
-Inductive SpecM (E : Type) `{EncodedType E} : call_stack -> Type@{entree_u} -> Type := 
-  | RetS Γ A (a : A) : SpecM E Γ A
-  | BindS Γ A B : SpecM E Γ A -> (A -> SpecM E Γ B) -> SpecM E Γ B
-  | IterS Γ A B : (A -> SpecM E Γ (A + B)) -> A -> SpecM E Γ B
-  | CallS Γ A B (a : A) : SpecM E (ct_intro A B :: Γ) (B a)
-  | MrecS Γ A B (bodies : forall a, SpecM E (ct_intro A B :: Γ) (B a) ) (a : A):
-    SpecM E Γ (B a)
-  | TriggerS Γ (e : E) : SpecM E Γ (encodes e)
-  | AssumeS Γ (P : Prop) : SpecM E Γ unit
-  | AssertS Γ (P : Prop) : SpecM E Γ unit
-  | ForallS Γ (A : Set) : SpecM E Γ A
-  | ExistsS Γ (A : Set) : SpecM E Γ A
-.
+
+
+
+
+
+
+
 (* I think there is an associativity issue here want + E to be at the top
    maybe the way to do that is have nil map to void and only add E at the top level
 *)
@@ -90,33 +340,7 @@ induction Γ.
 - simpl. intros e. apply IHΓ.
 Defined.
 
-Arguments RetS {_ _ _ _} _.
-Arguments BindS {_ _ _ _ _} _ _.
-Arguments IterS {_ _ _ _ _} _ _.
-Arguments AssumeS {_ _ _}.
-Arguments AssertS {_ _ _}.
-Arguments ExistsS {_ _ _}.
-Arguments ForallS {_ _ _}.
-Arguments CallS {_ _ _ _ _} _.
-Arguments MrecS {_ _ _} _ _ _ _.
-Arguments TriggerS {_ _ _} _.
 
-Fixpoint denote_SpecM (E : Type@{entree_u}) `{EncodedType E} Γ A (spec : SpecM E Γ A) : 
-  entree_spec (denote_call_stack E Γ) A :=
-  match spec with
-  | RetS a => Ret a
-  | BindS m k => EnTree.bind (denote_SpecM E _ _ m) (fun x => denote_SpecM E _ _ (k x))
-  | IterS body a => EnTree.iter (fun x => denote_SpecM E _ _ (body x)) a
-  | AssumeS P => assume_spec P
-  | AssertS P => assert_spec P
-  | ForallS A => forall_spec A
-  | ExistsS A => exists_spec A
-  | TriggerS e => trigger e
-  | CallS a => (EnTree.trigger (Spec_vis (inl (CallDep _ _ a))))
-  | MrecS A B bodies a => mrec_spec (fun c : call_depE _ _  => 
-                         match c with CallDep _ _ a => denote_SpecM E _ _ (bodies a) end) 
-                               (CallDep _ _ a)
-  end.
 
 
 #[global] Instance SpecM_Monad {E} `{EncodedType E} Γ : Monad (SpecM E Γ) :=
